basic defs for mutable references

dev2015/fsub3.v
@@ -6,6 +6,7 @@
 (* it also turns types into proper first class objects, *)
 (* compared to fsub1.v *)
 
+(* this version adds mutable references to fsub2.v *)
 
 (*
 TODO:
@@ -28,6 +29,7 @@ Inductive ty : Type :=
   | TTop   : ty    
   | TFun   : ty -> ty -> ty
   | TMem   : ty -> ty -> ty
+  | TCell  : ty -> ty
   | TSel   : id -> ty
   | TSelH  : id -> ty
   | TSelB  : id -> ty
@@ -39,6 +41,9 @@ Inductive tm : Type :=
   | tfalse : tm
   | tvar   : id -> tm
   | ttyp   : ty -> tm
+  | tnew   : ty -> tm
+  | tget   : tm -> tm
+  | tset   : tm -> tm -> tm
   | tapp   : tm -> tm -> tm (* f(x) *)
   | tabs   : id -> id -> tm -> tm (* \f x.y *)
   | ttapp  : tm -> tm -> tm (* f[X] *)
@@ -48,6 +53,7 @@ Inductive tm : Type :=
 Inductive vl : Type :=
 | vty   : list (id*vl) -> ty -> vl
 | vbool : bool -> vl
+| vloc  : id -> vl
 | vabs  : list (id*vl) -> id -> id -> tm -> vl
 | vtabs : list (id*vl) -> id -> ty -> tm -> vl
 .
@@ -110,6 +116,9 @@ Inductive closed_rec: nat -> nat -> ty -> Prop :=
     closed_rec k l T1 ->
     closed_rec k l T2 ->
     closed_rec k l (TMem T1 T2)
+| cl_cell: forall k l T1,
+    closed_rec k l T1 ->
+    closed_rec k l (TCell T1)
 | cl_bind: forall k l T1 T2,
     closed_rec k l T1 ->
     closed_rec (S k) l T2 ->
@@ -138,6 +147,7 @@ Fixpoint open_rec (k: nat) (u: ty) (T: ty) { struct T }: ty :=
     | TTop        => TTop
     | TBot        => TBot
     | TBool       => TBool
+    | TCell T1    => TCell (open_rec k u T1)
     | TMem T1 T2  => TMem (open_rec k u T1) (open_rec k u T2)
     | TFun T1 T2  => TFun (open_rec k u T1) (open_rec k u T2)
   end.
@@ -155,6 +165,7 @@ Fixpoint subst (U : ty) (T : ty) {struct T} : ty :=
     | TTop         => TTop
     | TBot         => TBot
     | TBool        => TBool
+    | TCell T1     => TCell (subst U T1)
     | TMem T1 T2   => TMem (subst U T1) (subst U T2)
     | TFun T1 T2   => TFun (subst U T1) (subst U T2)
     | TSelB i      => TSelB i
@@ -168,6 +179,7 @@ Fixpoint nosubst (T : ty) {struct T} : Prop :=
     | TTop         => True
     | TBot         => True
     | TBool        => True
+    | TCell T1     => nosubst T1
     | TMem T1 T2   => nosubst T1 /\ nosubst T2
     | TFun T1 T2   => nosubst T1 /\ nosubst T2
     | TSelB i      => True
@@ -194,6 +206,10 @@ Inductive stp: tenv -> tenv -> ty -> ty -> Prop :=
     stp G1 GH TBot T2
 | stp_bool: forall G1 GH,
     stp G1 GH TBool TBool
+| stp_cell: forall G1 GH T1 T2,
+    stp G1 GH T1 T2 ->
+    stp G1 GH T2 T1 ->
+    stp G1 GH (TCell T1) (TCell T2)
 | stp_fun: forall G1 GH T1 T2 T3 T4,
     stp G1 GH T3 T1 ->
     stp G1 GH T2 T4 ->
@@ -266,6 +282,16 @@ Inductive has_type : tenv -> tm -> ty -> Prop :=
 | t_typ: forall env T1,
            stp env [] T1 T1 ->
            has_type env (ttyp T1) (TMem T1 T1)
+| t_new: forall env T1,
+           stp env [] T1 T1 ->
+           has_type env (tnew T1) (TCell T1)
+| t_get: forall env T1 x,
+           has_type env x (TCell T1) ->
+           has_type env (tget x) T1
+| t_set: forall env T1 x y,
+           has_type env x (TCell T1) ->
+           has_type env y T1 ->
+           has_type env (tset x y) T1
 | t_app: forall env f x T1 T2,
            has_type env f (TFun T1 T2) ->
            has_type env x T1 ->
@@ -308,6 +334,7 @@ Definition base (v:vl): venv :=
   match v with
     | vty GX _ => GX
     | vbool _ => nil
+    | vloc _ => nil
     | vabs GX _ _ _ => GX
     | vtabs GX _ _ _ => GX
   end.
@@ -333,6 +360,10 @@ Inductive stp2: bool -> bool -> venv -> ty -> venv -> ty -> list (id*(venv*ty)) 
     stp2 false false G2 T3 G1 T1 GH n1 ->
     stp2 false false G1 T2 G2 T4 GH n2 ->
     stp2 m true G1 (TMem T1 T2) G2 (TMem T3 T4) GH (S (n1+n2))
+| stp2_cell: forall m G1 G2 T1 T2 GH n1 n2,
+    stp2 false false G2 T2 G1 T1 GH n1 ->
+    stp2 false false G1 T1 G2 T2 GH n2 ->
+    stp2 m true G1 (TCell T1) G2 (TCell T2) GH (S (n1+n2))
 
 
 (* strong version, with precise/invertible bounds *)
@@ -355,16 +386,16 @@ Inductive stp2: bool -> bool -> venv -> ty -> venv -> ty -> list (id*(venv*ty)) 
          
          
 (* existing object, but imprecise type *)
-| stp2_sel1: forall G1 G2 TX x T2 GH n1 v,
+| stp2_sel1: forall G1 G2 TX x T2 GH STO n1 v,
     index x G1 = Some v ->
-    val_type (base v) v TX ->
+    val_type STO (base v) v TX ->
     closed 0 0 TX ->
     stp2 false false (base v) TX G2 (TMem TBot T2) GH n1 ->
     stp2 false true G1 (TSel x) G2 T2 GH (S n1)
 
-| stp2_sel2: forall G1 G2 TX x T1 GH n1 v,
+| stp2_sel2: forall G1 G2 TX x T1 GH STO n1 v,
     index x G2 = Some v ->
-    val_type (base v) v TX ->           
+    val_type STO (base v) v TX ->           
     closed 0 0 TX ->
     stp2 false false (base v) TX G1 (TMem T1 TTop) GH n1 ->
     stp2 false true G1 T1 G2 (TSel x) GH (S n1)
@@ -412,34 +443,39 @@ Inductive stp2: bool -> bool -> venv -> ty -> venv -> ty -> list (id*(venv*ty)) 
 
 
 
-with wf_env : venv -> tenv -> Prop := 
-| wfe_nil : wf_env nil nil
-| wfe_cons : forall n v t vs ts,
-    val_type ((n,v)::vs) v t ->
-    wf_env vs ts ->
-    wf_env (cons (n,v) vs) (cons (n,t) ts)
+with wf_env : venv -> venv -> tenv -> Prop := 
+| wfe_nil : forall sto, wf_env sto nil nil
+| wfe_cons : forall sto n v t vs ts,
+    val_type sto ((n,v)::vs) v t ->
+    wf_env sto vs ts ->
+    wf_env sto (cons (n,v) vs) (cons (n,t) ts)
 
-with val_type : venv -> vl -> ty -> Prop :=
-| v_ty: forall env venv tenv T1 TE,
-    wf_env venv tenv -> (* T1 wf in tenv ? *)
+with val_type : venv -> venv -> vl -> ty -> Prop :=
+| v_ty: forall sto env venv tenv T1 TE,
+    wf_env sto venv tenv -> (* T1 wf in tenv ? *)
     (exists n, stp2 true true venv (TMem T1 T1) env TE [] n)->
-    val_type env (vty venv T1) TE
-| v_bool: forall venv b TE,
+    val_type sto env (vty venv T1) TE
+| v_bool: forall sto venv b TE,
     (exists n, stp2 true true [] TBool venv TE [] n) ->
-    val_type venv (vbool b) TE
-| v_abs: forall env venv tenv f x y T1 T2 TE,
-    wf_env venv tenv ->
+    val_type sto venv (vbool b) TE
+| v_loc: forall sto venv b v T1 TE,
+    index b sto = Some v ->
+    val_type sto sto v T1 ->       
+    (exists n, stp2 true true [] (TCell T1) venv TE [] n) ->
+    val_type sto venv (vloc b) TE
+| v_abs: forall sto env venv tenv f x y T1 T2 TE,
+    wf_env sto venv tenv ->
     has_type ((x,T1)::(f,TFun T1 T2)::tenv) y T2 ->
     fresh venv <= f ->
     1 + f <= x ->
     (exists n, stp2 true true venv (TFun T1 T2) env TE [] n)-> 
-    val_type env (vabs venv f x y) TE
-| v_tabs: forall env venv tenv x y T1 T2 TE,
-    wf_env venv tenv ->
+    val_type sto env (vabs venv f x y) TE
+| v_tabs: forall sto env venv tenv x y T1 T2 TE,
+    wf_env sto venv tenv ->
     has_type ((x,T1)::tenv) y (open (TSel x) T2) ->
     fresh venv = x ->
     (exists n, stp2 true true venv (TAll T1 T2) env TE [] n) ->
-    val_type env (vtabs venv x T1 y) TE
+    val_type sto env (vtabs venv x T1 y) TE
 .
 
 
@@ -506,18 +542,23 @@ Lemma stpd2_mem: forall G1 G2 GH T11 T12 T21 T22,
     stpd2 false G1 T12 G2 T22 GH ->
     stpd2 true G1 (TMem T11 T12) G2 (TMem T21 T22) GH.
 Proof. intros. repeat eu. eauto. Qed.
+Lemma stpd2_cell: forall G1 G2 GH T1 T2,
+    stpd2 false G2 T2 G1 T1 GH ->
+    stpd2 false G1 T1 G2 T2 GH ->
+    stpd2 true G1 (TCell T1) G2 (TCell T2) GH.
+Proof. intros. repeat eu. eauto. Qed.
 
-Lemma stpd2_sel1: forall G1 G2 TX x T2 GH v,
+Lemma stpd2_sel1: forall G1 G2 TX x T2 GH STO v,
     index x G1 = Some v ->
-    val_type (base v) v TX ->                
+    val_type STO (base v) v TX ->                
     closed 0 0 TX ->
     stpd2 false (base v) TX G2 (TMem TBot T2) GH ->
     stpd2 true G1 (TSel x) G2 T2 GH.
 Proof. intros. repeat eu. eauto. Qed.
 
-Lemma stpd2_sel2: forall G1 G2 TX x T1 GH v,
+Lemma stpd2_sel2: forall G1 G2 TX x T1 GH STO v,
     index x G2 = Some v ->
-    val_type (base v) v TX ->                
+    val_type STO (base v) v TX ->                
     closed 0 0 TX ->
     stpd2 false (base v) TX G1 (TMem T1 TTop) GH ->
     stpd2 true G1 T1 G2 (TSel x) GH.
